Splinter/Tables.i.dfy
@@ -104,7 +104,7 @@ module AllocationTableMachineMod refines MarshalledSnapshot {
     s1.table !! s2.table
   }
 
-  function Alloc(s: Variables) : set<AU> {
+  function Alloc(s: Variables) : set<CU> {
     {} // TODO
   }
 }
